speclib fixes

compiler/fstar-compiler/specs/speclib.fst
@@ -2,116 +2,196 @@ module Speclib
 open Lib.IntTypes
 open Lib.Sequence
 open Lib.ByteSequence
-
+open Lib.LoopCombinators
+open FStar.Mul
 inline_for_extraction type nat_t = nat
 inline_for_extraction type pos_t = pos
 
 type numeric = 
   | Word of inttype
+  | BV of n:size_nat{n > 0}
+  | NATm of n:nat{n > 1}
   | Int 
 
-inline_for_extraction let numeric_t (n:numeric) = 
+inline_for_extraction let numeric_t (n:numeric) : Type0 = 
   match n with
-  | Word i -> uint_t i
+  | Word i -> uint_t i PUB
+  | BV n -> x:nat{x < pow2 n}
+  | NATm n -> x:nat{x < n}
   | Int -> int
+
+inline_for_extraction let numeric_v (#n:numeric)  (x:numeric_t n) : int = 
+  match n with
+  | Word i -> uint_v (x <: uint_t i PUB)
+  | BV n -> x
+  | NATm n -> x
+  | Int -> x
 
 inline_for_extraction let zero (n:numeric) : numeric_t n = 
   match n with
-  | Word t -> nat_to_uint #t 0
+  | Word t -> nat_to_uint #t #PUB 0
+  | BV n -> 0
+  | NATm n -> 0
   | Int -> 0
 
 inline_for_extraction let one (n:numeric) : numeric_t n = 
   match n with
-  | Word t -> nat_to_uint #t 1
+  | Word t -> nat_to_uint #t #PUB 1
+  | BV n -> 1
+  | NATm n -> 1
   | Int -> 1
 
 inline_for_extraction let bitvector (n:numeric) = 
   match n with
-  | Word i -> machineint i
+  | Word i -> True
+  | BV n -> True
+  | NATm n -> False
   | Int -> False
 
 inline_for_extraction let comparable (n:numeric) = 
   match n with
-  | Word SIZE -> True
-  | Word (NATm _) -> True
+  | Word i -> True
+  | BV _ -> True
+  | NATm _ -> True
   | Int -> True
-  | _ -> False
 
 inline_for_extraction let divisible (n:numeric) = 
   match n with
-  | Word SIZE -> True
-  | Word (NATm _) -> True
+  | Word U128 -> False
+  | Word _ -> True
+  | BV n -> True
+  | NATm n -> True
   | Int -> True
-  | _ -> False
 
 inline_for_extraction let shiftval (n:numeric{bitvector n}) =
   match n with
-  | Word t -> n:nat{n < bits t} //shiftval t
+  | Word t -> shiftval t
+  | BV n -> x:size_t{uint_v x < n}
 
 inline_for_extraction let rotval (n:numeric{bitvector n}) =
   match n with
-  | Word t -> n:nat{n > 0 /\ n < bits t} //rotval t
+  | Word t -> rotval t
+  | BV n -> x:size_t{uint_v x > 0 /\ uint_v x < n}
 
 inline_for_extraction let (+.) (#n:numeric) (a:numeric_t n) (b:numeric_t n) : numeric_t n = 
   match n with
-  | Word t -> (a <: uint_t t) +. b
+  | Word t -> (a <: uint_t t PUB)  +. b
+  | BV n -> (a + b) % pow2 n
+  | NATm n -> (a + b) % n
   | Int -> a + b
 
 inline_for_extraction let (-.) (#n:numeric) (a:numeric_t n) (b:numeric_t n) : numeric_t n = 
   match n with
-  | Word t -> (a <: uint_t t) -. b
+  | Word t -> (a <: uint_t t PUB) -. b
+  | BV n -> (n + a - b) % pow2 n
+  | NATm n -> (n + a - b) % n
   | Int -> a - b
 
 inline_for_extraction let ( *. ) (#n:numeric{n <> Word U128}) (a:numeric_t n) (b:numeric_t n) : numeric_t n = 
   match n with
-  | Word t -> (a <: uint_t t) *. b
+  | Word t -> (a <: uint_t t PUB) *. b
+  | BV n -> (a `op_Multiply` b) % pow2 n
+  | NATm n -> (a `op_Multiply` b) % n
   | Int -> a `op_Multiply` b
 
-inline_for_extraction let (/.) (#n:numeric{divisible n}) (a:numeric_t n) (b:numeric_t n) : numeric_t n = 
+#reset-options "--z3rlimit 30"
+
+inline_for_extraction let (/.) (#n:numeric{divisible n}) (a:numeric_t n) (b:numeric_t n{numeric_v b > 0}) : numeric_t n = 
   match n with
-  | Word t -> (a <: uint_t t) /. b
+  | Word t -> (a <: uint_t t PUB) /. b
+  | BV n -> a / b
+  | NATm n -> a / b
   | Int -> a / b
 
-inline_for_extraction let (%.) (#n:numeric{divisible n}) (a:numeric_t n) (b:numeric_t n) : numeric_t n = 
+inline_for_extraction let (%.) (#n:numeric{divisible n}) (a:numeric_t n) (b:numeric_t n{numeric_v b > 0}) : numeric_t n = 
   match n with
-  | Word t -> (a <: uint_t t) %. b
+  | Word t -> (a <: uint_t t PUB) %. b
+  | BV n -> a % b
+  | NATm n -> a % b
   | Int -> a % b
 
 
 inline_for_extraction let ( <<. ) (#n:numeric{bitvector n}) (a:numeric_t n) (b:shiftval n) : numeric_t n = 
   match n with
-  | Word t -> (a <: uint_t t) <<. u32 b
+  | Word t -> (a <: uint_t t PUB) <<. b
+  | BV n -> (a `op_Multiply` pow2 (uint_v #U32 #PUB b)) % pow2 n
 
+
+#set-options "--z3rlimit 200 --max_fuel 3 --max_ifuel 5"
 inline_for_extraction let ( >>. ) (#n:numeric{bitvector n}) (a:numeric_t n) (b:shiftval n) : numeric_t n = 
   match n with
-  | Word t -> (a <: uint_t t) >>. u32 b
+  | Word t -> (a <: uint_t t PUB) >>. b
+  | BV n -> let a : (x:nat{x < pow2 n}) = a in
+	   let mv = uint_v #U32 #PUB b in
+           let x = a / pow2 mv in
+	   Math.Lemmas.lemma_div_lt a n mv;
+	   x
+
+let natm_to_bv (#n:size_nat{n > 0}) (x:nat{x < pow2 n}) : lseq bit_t n =  
+  createi n (fun i -> uint ((x / pow2 i) % 2)) 
+
+let bv_to_natm (#n:size_nat{n > 0}) (x:lseq bit_t n) : (x:nat{x < pow2 n}) = 
+  repeati_inductive #nat n 
+    (fun i a -> a < pow2 i)
+    (fun i a -> a + uint_v x.[i] * pow2 i) 0
 
 inline_for_extraction let ( &. ) (#n:numeric{bitvector n}) (a:numeric_t n) (b:numeric_t n) : numeric_t n = 
   match n with
-  | Word t -> (a <: uint_t t) &. b
-
+  | Word t -> (a <: uint_t t PUB) &. b
+  | BV n -> let a_bv = natm_to_bv #n a in
+	   let b_bv = natm_to_bv #n b in
+	   let c_bv = map2 ( &. ) a_bv b_bv in
+	   bv_to_natm #n c_bv
+    
 inline_for_extraction let ( |. ) (#n:numeric{bitvector n}) (a:numeric_t n) (b:numeric_t n) : numeric_t n = 
   match n with
-  | Word t -> (a <: uint_t t) |. b
-
+  | Word t -> (a <: uint_t t PUB) |. b
+  | BV n -> bv_to_natm #n (map2 ( |. ) (natm_to_bv a) (natm_to_bv b))
+  
 inline_for_extraction let ( ^. ) (#n:numeric{bitvector n}) (a:numeric_t n) (b:numeric_t n) : numeric_t n = 
   match n with
-  | Word t -> (a <: uint_t t) ^. b
+  | Word t -> (a <: uint_t t PUB) ^. b
+  | BV n -> bv_to_natm #n (map2 ( ^. ) (natm_to_bv a) (natm_to_bv b))
+
+inline_for_extraction let ( ~. ) (#n:numeric{bitvector n}) (a:numeric_t n) : numeric_t n = 
+  match n with
+  | Word t -> ~. (a <: uint_t t PUB) 
+  | BV n -> bv_to_natm #n (map ( ~. ) (natm_to_bv a))
+
+inline_for_extraction let ( <. ) (#n:numeric{comparable n}) (a:numeric_t n) (b:numeric_t n) : bool = 
+  match n with
+  | Word t -> (a <: uint_t t PUB) <. b
+  | BV n -> a < b
+  | NATm m -> a < b
+  | Int -> a < b
 
 inline_for_extraction let ( <=. ) (#n:numeric{comparable n}) (a:numeric_t n) (b:numeric_t n) : bool = 
   match n with
-  | Word t -> (a <: uint_t t) <=. b
+  | Word t -> (a <: uint_t t PUB) <=. b
+  | BV n -> a <= b
+  | NATm m -> a <= b
   | Int -> a <= b
 
 inline_for_extraction let ( =. ) (#n:numeric{comparable n}) (a:numeric_t n) (b:numeric_t n) : bool = 
   match n with
-  | Word t -> (a <: uint_t t) =. b
+  | Word t -> (a <: uint_t t PUB) =. b
+  | BV m -> a = b
+  | NATm m -> a = b
   | Int -> a = b
 
 inline_for_extraction let ( >. ) (#n:numeric{comparable n}) (a:numeric_t n) (b:numeric_t n) : bool = 
   match n with
-  | Word t -> (a <: uint_t t) >. b
+  | Word t -> (a <: uint_t t PUB) >. b
+  | BV m -> a > b
+  | NATm m -> a > b
   | Int -> a > b
+
+inline_for_extraction let ( >=. ) (#n:numeric{comparable n}) (a:numeric_t n) (b:numeric_t n) : bool = 
+  match n with
+  | Word t -> (a <: uint_t t PUB) >=. b
+  | BV m -> a >= b
+  | NATm m -> a >= b
+  | Int -> a >= b
 
 inline_for_extraction let rec exp  (#n:numeric{n <> Word U128}) (x:numeric_t n) (y:nat) : numeric_t n = 
     if y = 0 then one n 
@@ -126,39 +206,47 @@ inline_for_extraction let ( **. ) (#n:numeric{n <> Word U128}) (x:numeric_t n) (
     if n = Int && x = 2 then pow2 y
     else exp #n x y
 
-inline_for_extraction let natmod_t (n:pos) = numeric_t (Word (NATm n))
+inline_for_extraction let natmod_t (n:nat{n > 1}) = numeric_t (NATm n)
 inline_for_extraction let natmod n p : natmod_t p = n % p
-inline_for_extraction let natmod_to_nat (#m:pos) (a:natmod_t m) : x:nat{x < m}  = a
-inline_for_extraction let natmod_to_int (#m:pos) (a:natmod_t m) : x:nat{x < m}  = a
+inline_for_extraction let natmod_to_nat (#m:nat{m > 1}) (a:natmod_t m) : x:nat{x < m}  = a
+inline_for_extraction let natmod_to_int (#m:nat{m > 1}) (a:natmod_t m) : x:nat{x < m}  = a
 
-inline_for_extraction let uintn_t (n:nat) = numeric_t (Word (NATm (pow2 n)))
-inline_for_extraction let bit_t:eqtype = numeric_t (Word (NATm 2))
+inline_for_extraction let uintn_t (n:pos) = numeric_t (NATm (pow2 n))
+inline_for_extraction let uint1_t = numeric_t (Word U1)
 inline_for_extraction let uint8_t = numeric_t (Word U8)
+inline_for_extraction let uint16_t = numeric_t (Word U16)
 inline_for_extraction let uint32_t = numeric_t (Word U32)
 inline_for_extraction let uint64_t = numeric_t (Word U64)
 inline_for_extraction let uint128_t = numeric_t (Word U128)
 
 inline_for_extraction let uintn n p : uintn_t p = natmod n (pow2 p)
-inline_for_extraction let bit x : bit_t = modulo x 2
-inline_for_extraction let uint8 x : uint8_t = u8 (x % (pow2 8))
-inline_for_extraction let uint32 x : uint32_t = u32 (x % (pow2 32))
-inline_for_extraction let uint64 x : uint64_t = u64 (x % (pow2 64))
-inline_for_extraction let uint128 x : uint128_t = u128 (x % (pow2 128))
+inline_for_extraction let bit x : bit_t = uint #U1 #PUB (x % 2)
+inline_for_extraction let uint8 x : uint8_t = uint #U8 #PUB  (x % pow2 8)
+inline_for_extraction let uint16 x : uint16_t = uint #U16 #PUB  (x % pow2 16)
+inline_for_extraction let uint32 x : uint32_t = uint #U32 #PUB  (x % pow2 32)
+inline_for_extraction let uint64 x : uint64_t = uint #U64 #PUB  (x % pow2 64)
+inline_for_extraction let uint128 x : uint128_t = uint #U128 #PUB  (x % pow2 128)
 
-inline_for_extraction let uintn_to_nat #n (a:numeric_t n) : nat =
+inline_for_extraction let uintn_to_int #n (a:numeric_t n) : int =
   match n with
-  | Word t -> Lib.RawIntTypes.uint_to_nat #t a
+  | Word t -> pub_int_v #t a
+  | BV m -> a
+  | NATm m -> a
   | Int -> a
   
-inline_for_extraction let uintn_to_int #n (a:numeric_t n) : nat = uintn_to_nat #n a
-inline_for_extraction let uintn_get_bit #n (x:numeric_t n) (i:nat) : bit_t = 
+inline_for_extraction let uintn_to_nat #n (a:numeric_t n{numeric_v a >= 0}) : nat = uintn_to_int #n a
+
+inline_for_extraction let uintn_get_bit #n (x:numeric_t n) (i:size_nat) : bit_t = 
   match n with
-  | Word (NATm m) ->  bit (((uintn_to_nat #n x) / pow2 i) % 2)
-  | Word _ -> bit ((uintn_to_nat (x >>. i)) % 2)
+  | Word t -> if i < bits t then bit ((uintn_to_nat (x >>. size i)) % 2) else bit 0
+  | BV m ->  bit (((uintn_to_nat #n x) / pow2 i) % 2)
+  | NATm m ->  bit (((uintn_to_nat #n x) / pow2 i) % 2)
   | Int -> bit ((x % pow2 i) % 2)
   
-inline_for_extraction let uintn_rotate_left (#t:m_inttype) (a:uint_t t) b = a <<<. (u32 b)
-inline_for_extraction let uintn_rotate_right (#t:m_inttype) (a:uint_t t) b = a >>>. (u32 b)
+inline_for_extraction let uintn_rotate_left (#t:inttype) (a:uint_t t PUB) (b:Lib.IntTypes.rotval t) : uint_t t PUB = a <<<. b
+
+inline_for_extraction let uintn_rotate_right (#t:inttype) (a:uint_t t PUB) (b:Lib.IntTypes.rotval t) : uint_t t PUB = a >>>. b
+
 
 type result_t (t:Type0) = 
   | Retval of t
@@ -166,14 +254,14 @@ type result_t (t:Type0) =
 inline_for_extraction let result_retval #t (x:t) : result_t t = Retval x
 inline_for_extraction let result_error #t (x:string) : result_t t = Error x
 
-inline_for_extraction let range_t min max = n:nat{n >= min /\ n < max}
+inline_for_extraction let range_t min max = n:size_t{v n >= min /\ v n < max}
 unfold let range i = i
 inline_for_extraction let repeati = repeati
 
-inline_for_extraction let array_t t len = lseq t len
-inline_for_extraction let vlarray_t t = seq t
+unfold inline_for_extraction let array_t t len = lseq t len
+unfold inline_for_extraction let vlarray_t t = seq t
 inline_for_extraction let array x = x
-inline_for_extraction let array_length a = length a
+inline_for_extraction let array_length a : numeric_t Int = length a
 inline_for_extraction let array_copy #a #l (x:array_t a l) : array_t a l = x
 inline_for_extraction let op_String_Access #a #len = index #a #len
 inline_for_extraction let op_String_Assignment #a #len = upd #a #len
@@ -181,36 +269,64 @@ inline_for_extraction let array_createL l = createL l
 inline_for_extraction let array_create x y = create x y
 inline_for_extraction let array_slice #l (x:lseq 'a l) y z = slice x y z
 inline_for_extraction let array_update_slice #l (x:lseq 'a l) y z w = update_slice x y z w
-inline_for_extraction val array_split_blocks: #a:Type -> s:seq a -> bs:size_nat{bs > 0} -> (bl:lseq (lseq a bs) (length s / bs) * l:lseq a (length s % bs))
+
+
+inline_for_extraction val array_split_blocks: #a:Type -> 
+  s:seq a -> bs:nat{bs > 0 /\ bs <= max_size_t /\ length s / bs <= max_size_t} -> 
+  (lseq (lseq a bs) (length s / bs) & lseq a (length s % bs))
 inline_for_extraction let array_split_blocks #a s bs = 
-    let nblocks = length s / bs in
-    let rem = length s % bs in
-    let blocks = create nblocks (create bs (u8 0)) in
-    repeati nblocks (fun i blocks -> blocks.[i] <- sub (to_lseq s) (i `op_Multiply` bs) bs) blocks,
-    sub (to_lseq s) (length s - rem) rem 
+    let len = length s in
+    let nblocks : size_nat = len / bs in
+    let rem : size_nat = len % bs in
+    assert (nblocks * bs <= len);
+    let blocks = createi #(lseq a bs) nblocks
+      (fun i -> assert (i + 1 <= nblocks);
+	     assert ((i + 1) * bs <= len); 
+	     assert (i * bs <= (i + 1) * bs); 
+	     let j:n:nat{i * bs <= n /\ n <= len} = (i+1) * bs in
+	     Seq.slice s (i * bs) j) in //(i*bs + bs)) in
+    let last : lseq a rem = Seq.slice s (len - rem) len  in
+    (blocks, last)
     
-inline_for_extraction val array_concat_blocks: #a:Type -> #n:size_nat -> #bs:size_nat{bs > 0} -> bl:lseq (lseq a bs) n -> l:seq a -> r:lseq a (n `op_Multiply` bs + length l)
-inline_for_extraction let array_concat_blocks #a #n #bs bl l = 
-    let msg = create (n `op_Multiply` bs + length l) (u8 0) in
-    let msg = repeati n (fun i msg -> update_sub msg (i `op_Multiply` bs) bs bl.[i]) msg in
-    update_sub msg (n `op_Multiply` bs) (length l) l
+    
+inline_for_extraction val array_concat_blocks: 
+  #a:Type -> #n:size_nat -> #bs:size_nat{bs > 0} -> #rem:size_nat{n * bs + rem <= max_size_t} -> 
+  bl:lseq (lseq a bs) n -> 
+  l:lseq a rem -> 
+  r:lseq a (n * bs + rem)
+inline_for_extraction let array_concat_blocks #a #n #bs #rem bl l = 
+  createi (n * bs + rem) 
+    (fun i -> if i < n * bs then 
+	      (bl.[i / bs]).[i % bs]
+	   else l.[i - (n * bs)])
+    
 
-
-inline_for_extraction let bytes_t len = lbytes len
-inline_for_extraction let vlbytes_t = bytes
+unfold inline_for_extraction let bytes_t len = lseq uint8_t len
+unfold inline_for_extraction let vlbytes_t = seq uint8_t
 inline_for_extraction let bytes x = x
 inline_for_extraction let bytes_copy x = x
 inline_for_extraction let bytes_length x = length x
-inline_for_extraction let bytes_to_uint32s_le #l (b:lbytes (l `op_Multiply` 4)) = uints_from_bytes_le #U32 #l b
-inline_for_extraction let bytes_from_uint32s_le #l (b:lseq uint32_t l) = uints_to_bytes_le #U32 b 
-inline_for_extraction let bytes_to_nat_le #l (b:lbytes l) = nat_from_bytes_le #l b
-inline_for_extraction let bytes_from_nat_le (n:nat) l = nat_to_bytes_le l n
-inline_for_extraction let bytes_to_uint64_le #l (b:lbytes l) = uint_from_bytes_le #U64 b
-inline_for_extraction let bytes_from_uint64_le (n:uint64_t) = uint_to_bytes_le #U64 n
-inline_for_extraction let bytes_to_uint128_le #l (b:lbytes l) = uint_from_bytes_le #U128 b
-inline_for_extraction let bytes_from_uint128_le (n:uint128_t) = uint_to_bytes_le #U128 n
-inline_for_extraction let bytes_to_uint128_be #l (b:lbytes l) = uint_from_bytes_be #U128 b
-inline_for_extraction let bytes_from_uint128_be (n:uint128_t) = uint_to_bytes_be #U128 n
-inline_for_extraction let bytes_to_uint32_be #l (b:lbytes l) = uint_from_bytes_be #U32 b
-inline_for_extraction let bytes_from_uint32_be (n:uint32_t) = uint_to_bytes_be #U32 n
+inline_for_extraction let bytes_to_nat_le #l (b:bytes_t l) = nat_from_bytes_le b
+inline_for_extraction let bytes_from_nat_le (n:nat) (l:nat{n < pow2 (8 * l)}) = nat_to_bytes_le #PUB l n
+
+inline_for_extraction let bytes_to_uint32s_le (#l:size_nat{l * 4 <= max_size_t})
+		      (b:bytes_t (l * 4)) = uints_from_bytes_le #U32 #PUB #l b
+inline_for_extraction let bytes_from_uint32s_le (#l:size_nat{l * 4 <= max_size_t}) (b:lseq uint32_t l) : bytes_t (l*4) = uints_to_bytes_le #U32 b 
+inline_for_extraction let bytes_to_uint32s_be (#l:size_nat{l * 4 <= max_size_t})
+		      (b:bytes_t (l * 4)) = uints_from_bytes_be #U32 #PUB #l b
+inline_for_extraction let bytes_from_uint32s_be (#l:size_nat{l * 4 <= max_size_t}) (b:lseq uint32_t l) : bytes_t (l*4) = uints_to_bytes_be #U32 b 
+
+inline_for_extraction let bytes_to_uint64s_le (#l:size_nat{l * 8 <= max_size_t})
+		      (b:bytes_t (l * 8)) = uints_from_bytes_le #U64 #PUB #l b
+inline_for_extraction let bytes_from_uint64s_le (#l:size_nat{l * 8 <= max_size_t}) (b:lseq uint64_t l) : bytes_t (l*8) = uints_to_bytes_le #U64 b 
+inline_for_extraction let bytes_to_uint64s_be (#l:size_nat{l * 8 <= max_size_t})
+		      (b:bytes_t (l * 8)) = uints_from_bytes_be #U64 #PUB #l b
+inline_for_extraction let bytes_from_uint64s_be (#l:size_nat{l * 8 <= max_size_t}) (b:lseq uint64_t l) : bytes_t (l*8) = uints_to_bytes_be #U64 b 
+
+inline_for_extraction let bytes_to_uint128s_le (#l:size_nat{l * 16 <= max_size_t})
+		      (b:bytes_t (l * 16)) = uints_from_bytes_le #U128 #PUB #l b
+inline_for_extraction let bytes_from_uint128s_le (#l:size_nat{l * 16 <= max_size_t}) (b:lseq uint128_t l) : bytes_t (l*16) = uints_to_bytes_le #U128 b 
+inline_for_extraction let bytes_to_uint128s_be (#l:size_nat{l * 16 <= max_size_t})
+		      (b:bytes_t (l * 16)) = uints_from_bytes_be #U128 #PUB #l b
+inline_for_extraction let bytes_from_uint128s_be (#l:size_nat{l * 16 <= max_size_t}) (b:lseq uint128_t l) : bytes_t (l*16) = uints_to_bytes_be #U128 b 
 
